MoreList.thy
@@ -1,0 +1,34 @@
+theory MoreList
+imports Main
+begin
+
+lemma filter':
+  assumes "filter P xs = ys1 @ [y] @ ys2" "y \<notin> set (ys1 @ ys2)"
+  assumes "\<forall> x \<in> set xs. P x \<and> x \<noteq> y \<longleftrightarrow> P' x"
+  shows "filter P' xs = ys1 @ ys2"
+  using assms
+proof-
+  have "filter (\<lambda>x. x \<noteq> y) ys1 = ys1"
+    using assms(2)
+    by (induction ys1, auto)
+  moreover
+  have "filter (\<lambda>x. x \<noteq> y) ys2 = ys2"
+    using assms(2)
+    by (induction ys2, auto)
+  moreover
+  have "filter P' xs = filter (\<lambda>x. P x \<and> x \<noteq> y) xs"
+  proof (rule filter_cong)
+    fix x
+    assume "x \<in> set xs" then 
+    show "P' x \<longleftrightarrow> P x \<and> x \<noteq> y"
+      using assms
+      by simp
+  qed simp
+  then have "filter P' xs = filter (\<lambda> x. x \<noteq> y) (filter P xs)"
+    by simp
+  ultimately show ?thesis
+    using assms \<open>y \<notin> set (ys1 @ ys2)\<close>
+    by auto
+qed
+
+end
